WIP: update label_hm_rel definition to include well-formedness

viper-total-heaps/ViperBoogieBasicRel.thy
@@ -591,7 +591,8 @@ definition label_rel :: "(vname \<Rightarrow> 'a total_state \<Rightarrow> ('a v
 definition label_hm_rel :: "ViperLang.program \<Rightarrow>  var_context \<Rightarrow> 'a ty_repr_bpl \<Rightarrow> (field_ident \<rightharpoonup> vname) \<Rightarrow> label_hm_repr_bpl \<Rightarrow> 'a total_trace \<Rightarrow> ('a vbpl_absval) nstate \<Rightarrow> bool"
   where "label_hm_rel Pr \<Lambda> TyRep FieldTr LabelMap t ns \<equiv>
              label_rel (\<lambda>h \<phi>. heap_var_rel Pr \<Lambda> TyRep FieldTr h (get_hh_total \<phi>)) (fst LabelMap) t ns
-          \<and>  label_rel (\<lambda>m \<phi>. mask_var_rel Pr \<Lambda> TyRep FieldTr m (get_mh_total \<phi>)) (snd LabelMap) t ns"
+          \<and>  label_rel (\<lambda>m \<phi>. mask_var_rel Pr \<Lambda> TyRep FieldTr m (get_mh_total \<phi>)) (snd LabelMap) t ns
+          \<and>  (\<forall> lbl \<phi>. t lbl = Some \<phi> \<longrightarrow> wf_mask_simple (get_mh_total \<phi>))"
             (*(\<exists>\<phi>. t lbl = Some \<phi> \<and>                  
                  heap_var_rel Pr \<Lambda> TyRep FieldTr (fst hm) (get_hh_total \<phi>) ns \<and>
                  mask_var_rel Pr \<Lambda> TyRep FieldTr (snd hm) (get_mh_total \<phi>) ns))"*)
